mark_bi, mark_bi_dag and spanning tree is done. Only union find is left.

sample_mark/verif_copy_bi.v
@@ -1,6 +1,4 @@
 Require Import RamifyCoq.lib.Coqlib.
-Require Import RamifyCoq.lib.EquivDec_ext.
-Require Export VST.floyd.proofauto.
 Require Import RamifyCoq.sample_mark.env_copy_bi.
 Require Import RamifyCoq.graph.graph_model.
 Require Import RamifyCoq.graph.weak_mark_lemmas.
@@ -13,10 +11,13 @@ Require Import RamifyCoq.msl_application.Graph_Copy.
 Require Import RamifyCoq.msl_application.GraphBi.
 Require Import RamifyCoq.msl_application.GraphBi_Copy.
 Require Import RamifyCoq.sample_mark.spatial_graph_bi_copy.
+Require Import VST.msl.wand_frame.
+Require Import VST.floyd.reassoc_seq.
+Require Import VST.floyd.field_at_wand.
 
-Local Open Scope logic.
+(* Local Open Scope logic. *)
 
-Hint Rewrite eval_cast_neutral_is_pointer_or_null using auto : norm. (* TODO: should not need this *)
+(* Hint Rewrite eval_cast_neutral_is_pointer_or_null using auto : norm. (* TODO: should not need this *) *)
 
 Local Coercion Graph_LGraph: Graph >-> LGraph.
 Local Coercion LGraph_SGraph: LGraph >-> SGraph.
@@ -30,30 +31,6 @@ Notation holegraph sh x g := (@vertices_at _ _ _ _ _ _ (@SGP pSGG_VST addr (addr
 Notation Graph := (@Graph pSGG_VST (@addr pSGG_VST) (addr * LR) unit).
 Notation vmap := (@LocalGraphCopy.vmap addr (addr * LR) addr (addr * LR) _ _ _ _ _ _ _ _ (@GMS _ _ _ CCS)).
 Existing Instances MGS biGraph maGraph finGraph RGF.
-
-(*
-Definition natural_alignment := 8.
-
-Definition malloc_compatible (n: Z) (p: val) : Prop :=
-  match p with
-  | Vptr b ofs => (natural_alignment | Int.unsigned ofs) /\
-                           Int.unsigned ofs + n < Int.modulus
-  | _ => False
-  end.
-
-Definition mallocN_spec :=
- DECLARE _mallocN
-  WITH n: Z
-  PRE [ 1%positive OF tint]
-     PROP (4 <= n <= Int.max_unsigned) 
-     LOCAL (temp 1%positive (Vint (Int.repr n)))
-     SEP ()
-  POST [ tptr tvoid ] 
-     EX v: val,
-     PROP (malloc_compatible n v) 
-     LOCAL (temp ret_temp v) 
-     SEP (memory_block Tsh n v).
-*)
 
 Definition mallocN_spec :=
  DECLARE _mallocN
@@ -87,79 +64,61 @@ Definition copy_spec :=
 
 Definition main_spec :=
  DECLARE _main
-  WITH u : unit
+  WITH u : globals
   PRE  [] main_pre prog nil u
   POST [ tint ] main_post prog nil u.
 
-Definition Vprog : varspecs := (_x, tptr (Tstruct _Node noattr))::(_y, tptr (Tstruct _Node noattr))::(_n, (Tstruct _Node noattr))::nil.
+Definition Gprog : funspecs := ltac:(with_library prog [copy_spec; mallocN_spec; main_spec]).
 
-Definition Gprog : funspecs := copy_spec :: mallocN_spec :: main_spec::nil.
+Lemma graph_local_facts: forall sh x (g: Graph), weak_valid g x -> graph sh x g |-- valid_pointer (pointer_val_val x).
+Proof.
+  intros. destruct H.
+  - simpl in H. subst x. entailer!.
+  - destruct (vgamma g x) as [[d l] r] eqn:?.
+    eapply derives_trans; [apply (@root_stable_ramify _ (sSGG_VST sh) g x _ Heqp); auto |].
+    Transparent sSGG_VST. simpl vertex_at at 1. entailer!. Opaque sSGG_VST.
+Qed.
 
-Lemma ADMIT: forall P: Prop, P.
-Admitted.
-
-Lemma body_mark: semax_body Vprog Gprog f_copy copy_spec.
+Lemma body_copy: semax_body Vprog Gprog f_copy copy_spec.
 Proof.
   start_function.
   remember (vgamma g x) as dlr eqn:?H.
   destruct dlr as [[d l] r].
   rename H0 into H_GAMMA_g; symmetry in H_GAMMA_g.
   rename H into H_weak_valid.
-  forward_if_tac  (* if (x == 0) *)
+  forward_if  (* if (x == 0) *)
     (PROP  (pointer_val_val x <> nullval)
      LOCAL (temp _x (pointer_val_val x))
      SEP   (graph sh x g)).
-  apply ADMIT. (* type checking for pointer comparable. VST will fix it. *)
-  Focus 1. { (* if-then branch *)
-    destruct_pointer_val x.
-    forward. (* return 0; *)
-    apply (exp_right ((NullPointer, g), empty_Graph)).
-    simpl.
-    entailer!; auto.
+  - apply denote_tc_test_eq_split. 2: entailer!. apply graph_local_facts; auto.
+  - assert (x = NullPointer) by (destruct x; simpl in H; inversion H; auto). subst x.
+    forward.
+    Exists ((NullPointer, g), empty_Graph).
+    simpl. entailer!.
     + apply (copy_null_refl g).
-    + rewrite va_reachable_invalid; auto.
-  } Unfocus.
-  Focus 1. { (* if-else branch *)
-    forward. (* skip; *)
-    entailer!.
-  } Unfocus.
-  normalize.
-  assert (vvalid g x) as gx_vvalid.
-  Focus 1. {
-    destruct H_weak_valid; [| auto].
-    simpl in H0.
-    subst; exfalso; apply H. auto.
-  } Unfocus.
-  destruct_pointer_val x. clear H0 H_weak_valid.
-
-  localize
-   (PROP  ()
-    LOCAL (temp _x (pointer_val_val x))
-    SEP   (data_at sh node_type (pointer_val_val d, (pointer_val_val l, pointer_val_val r))
-              (pointer_val_val x))).
-  (* localize *)
-
-  eapply semax_ram_seq;
-    [ subst RamFrame RamFrame0; unfold abbreviate;
-      repeat apply eexists_add_stats_cons; constructor
-    | load_tac
-    | abbreviate_semax_ram].
-  (* x0 = x -> m; *)
-
-  unlocalize (PROP ()  LOCAL  (temp _x0 (pointer_val_val d); temp _x (pointer_val_val x))  SEP  (graph sh x g)).
-
-  Grab Existential Variables.
-  Focus 2. {
-    simplify_ramif.
-    apply (@root_stable_ramify _ (sSGG_VST sh) g x _ H_GAMMA_g); auto.
-  } Unfocus.
-  (* unlocalize *)
-
-  unfold semax_ram.
-  forward_if_tac  (* if (x0 != 0) *)
-    (PROP   (d = null)
-     LOCAL (temp _x (pointer_val_val x))
-     SEP   (graph sh x g)).
+    + rewrite va_reachable_invalid; auto. apply derives_refl. (* TODO why?*)
+  - forward. entailer!.
+  - Intros.
+    assert (vvalid g x) as gx_vvalid. {
+      destruct H_weak_valid; [| auto]. simpl in H0.
+      subst; exfalso; apply H; auto.
+    } assert (isptr (pointer_val_val x) /\ exists b i, x = ValidPointer b i). {
+      destruct x. 2: exfalso; apply H; reflexivity. split; simpl; auto.
+      exists b, i. reflexivity.
+    } destruct H0 as [? [b [i ?]]]. clear H0 H_weak_valid.
+    localize [data_at sh node_type (pointer_val_val d, (pointer_val_val l, pointer_val_val r)) (pointer_val_val x)].
+    forward. (* x0 = x -> m; *) 1: entailer!; destruct d; simpl; auto.
+    unlocalize [graph sh x g]. 1: apply (@root_stable_ramify _ (sSGG_VST sh) g x _ H_GAMMA_g); auto.
+    forward_if  (* if (x0 != 0) *)
+      (PROP (d = null)
+       LOCAL (temp _x (pointer_val_val x))
+       SEP (graph sh x g)).
+    + apply denote_tc_test_eq_split. 2: entailer!.
+      eapply derives_trans; [apply (@root_stable_ramify _ (sSGG_VST sh) g (ValidPointer b i) _ H_GAMMA_g); auto |].
+      apply sepcon_valid_pointer1. Transparent sSGG_VST. simpl vertex_at. unfold_data_at 1%nat.
+      do 2 apply sepcon_valid_pointer1. pose proof (field_at_valid_ptr sh node_type [StructField _m] (pointer_val_val d) (Vptr b i)).
+      rewrite field_at_data_at. unfold node_type. simpl field_address.
+      simpl field_address in H1.
   apply ADMIT. (* type checking for pointer comparable. VST will fix it. *)
   Focus 1. { (* if-then branch *)
     forward. (* return x0; *)
