sample_mark/verif_dispose_bi.v
@@ -1,4 +1,3 @@
-Require Import VST.floyd.proofauto.
 Require Import RamifyCoq.sample_mark.env_dispose_bi.
 Require Import RamifyCoq.graph.graph_model.
 Require Import RamifyCoq.graph.path_lemmas.
@@ -14,9 +13,9 @@ Require Import RamifyCoq.floyd_ext.share.
 Require RamifyCoq.graph.weak_mark_lemmas.
 Import RamifyCoq.graph.weak_mark_lemmas.WeakMarkGraph.
 
-Local Open Scope logic.
-
-Arguments SingleFrame' {l} {g} {s}.
+Require Import VST.msl.wand_frame.
+Require Import VST.floyd.reassoc_seq.
+Require Import VST.floyd.field_at_wand.
 
 Local Coercion Graph_LGraph: Graph >-> LGraph.
 Local Coercion LGraph_SGraph: LGraph >-> SGraph.
@@ -70,17 +69,39 @@ Definition dispose_spec :=
 
 Definition main_spec :=
  DECLARE _main
-  WITH u : unit
-  PRE  [] main_pre prog nil u
-  POST [ tint ] main_post prog nil u.
+  WITH gv : globals
+  PRE  [] main_pre prog nil gv
+  POST [ tint ] main_post prog nil gv.
 
-Definition Vprog : varspecs := nil.
+Definition Gprog : funspecs := ltac:(with_library prog [mark_spec ; spanning_spec ; dispose_spec ; main_spec]).
 
-Definition Gprog : funspecs := mark_spec :: spanning_spec :: dispose_spec :: main_spec::nil.
+Lemma graph_local_facts: forall sh x (g: Graph), vvalid g x -> @derives mpred Nveric (graph sh x g) (valid_pointer (pointer_val_val x)).
+Proof.
+  intros.
+  eapply derives_trans; [apply (@va_reachable_root_stable_ramify pSGG_VST _ _ _ (sSGG_VST sh) g x (vgamma g x)); auto |].
+  simpl vertex_at. unfold trinode. entailer!.
+Qed.
 
-Lemma ADMIT: forall P: Prop, P.
-Admitted.
+Lemma graph_left_local_facts: forall sh x (g: Graph) d l r, vvalid g x -> vgamma g x = (d, l, r) -> graph sh x g |-- valid_pointer (pointer_val_val l).
+Proof.
+  intros.
+  eapply derives_trans; [apply (@graph_ramify_aux1_left pSGG_VST (sSGG_VST sh) g x d l r); auto | ].
+  assert (weak_valid g l) by (apply (gamma_left_weak_valid g x d l r); auto). destruct H1.
+  - simpl in H1. subst l. simpl pointer_val_val. apply sepcon_valid_pointer1. entailer!.
+  - apply sepcon_valid_pointer1. apply graph_local_facts; auto.
+Qed.
 
+Lemma graph_right_local_facts: forall sh x (g1 g2: Graph) l l' r,
+    vvalid g1 x -> vgamma g1 x = (true, l, r) -> vvalid g2 x -> vgamma g2 x = (true, l', r) -> edge_spanning_tree g1 (x, L) g2 ->
+    vertices_at sh (reachable g1 x) g2 |-- valid_pointer (pointer_val_val r).
+Proof.
+  intros.
+  eapply derives_trans; [apply (@graph_ramify_aux1_right pSGG_VST (sSGG_VST sh) g1 g2 x l r); auto | ].
+  assert (weak_valid g2 r) by (apply (gamma_right_weak_valid g2 x true l' r); auto). destruct H4.
+  - simpl in H4. subst r. simpl pointer_val_val. apply sepcon_valid_pointer1. entailer!.
+  - apply sepcon_valid_pointer1. apply graph_local_facts; auto.
+Qed.
+  
 Lemma body_spanning: semax_body Vprog Gprog f_spanning spanning_spec.
 Proof.
   start_function.
@@ -93,466 +114,179 @@ Proof.
     apply (valid_not_null g) in H. exfalso; auto.
     reflexivity.
   }
-  localize
-   (PROP  ()
-    LOCAL (temp _x (pointer_val_val x))
-    SEP   (data_at sh node_type (Vint (Int.repr 0), (pointer_val_val l, pointer_val_val r))
-                     (pointer_val_val x))).
-  
-  (* begin l = x -> l; *)
-  apply -> ram_seq_assoc.
-  eapply semax_ram_seq;
-    [ subst RamFrame RamFrame0; unfold abbreviate;
-      repeat apply eexists_add_stats_cons; constructor
-    | load_tac 
-    | abbreviate_semax_ram].
-  (* end l = x -> l; *)
-
-  (* begin r = x -> r; *)
-  apply -> ram_seq_assoc.
-  eapply semax_ram_seq;
-    [ subst RamFrame RamFrame0; unfold abbreviate;
-      repeat apply eexists_add_stats_cons; constructor
-    | load_tac 
-    | abbreviate_semax_ram].
-  (* end r = x -> r; *)
-
-  (* begin x -> m = 1; *)
-  apply -> ram_seq_assoc.
-  eapply semax_ram_seq;
-    [ subst RamFrame RamFrame0; unfold abbreviate;
-      repeat apply eexists_add_stats_cons; constructor
-    | store_tac
-    | abbreviate_semax_ram].
-  cbv beta zeta iota delta [replace_nth].
-  change (@field_at CompSpecs sh node_type []
-           (Vint (Int.repr 1), (pointer_val_val l, pointer_val_val r))) with
-         (@data_at CompSpecs sh node_type
-                   (Vint (Int.repr 1), (pointer_val_val l, pointer_val_val r))).
-  (* end x -> m = 1; *)
-  
-  unlocalize (PROP ()
-              LOCAL  (temp _r (pointer_val_val r); temp _l (pointer_val_val l); temp _x (pointer_val_val x))
-              SEP  (graph sh x (Graph_vgen g x true))).
-  Grab Existential Variables.
-  Focus 2. {
-    simplify_ramif.
+  localize [data_at sh node_type (Vint (Int.repr 0), (pointer_val_val l, pointer_val_val r))
+                    (pointer_val_val x)].
+  forward. 1: entailer!; destruct l; simpl; auto.
+  forward. 1: entailer!; destruct r; simpl; auto.
+  forward.
+  unlocalize [graph sh x (Graph_vgen g x true)].
+  Focus 1. {
     apply (@root_update_ramify _ (sSGG_VST sh) g x _ (false, l, r) (true, l, r)); auto.
     eapply Graph_vgen_vgamma; eauto.
   } Unfocus.
-
   (* if (l) { *)
-  apply -> ram_seq_assoc.
   symmetry in H1.
   pose proof Graph_vgen_true_mark1 g x _ _ H1 H.
   assert (H_GAMMA_g1: vgamma (Graph_vgen g x true) x = (true, l, r)) by
    (eapply Graph_vgen_vgamma; eauto).
-  assert (vvalid (Graph_vgen g x true) x) by (destruct H2 as [[? _] _]; apply H2; auto).
+  assert (vvalid (Graph_vgen g x true) x) by
+      (destruct H2 as [[? _] _]; apply H2; auto).
   forget (Graph_vgen g x true) as g1.
-  unfold semax_ram.
-  
-  forward_if_tac
-    (EX g2: Graph,
-     PROP  (edge_spanning_tree g1 (x, L) g2)
-     LOCAL (temp _r (pointer_val_val r);
-            temp _l (pointer_val_val l);
-            temp _x (pointer_val_val x))
-     SEP (vertices_at sh (reachable g1 x) g2)); [  apply ADMIT (* type checking for pointer comparable. VST will fix it. *)
- | | gather_current_goal_with_evar ..].
-
-  (* root_mark = l -> m; *)
-  localize
-    (PROP  ()
-     LOCAL (temp _l (pointer_val_val l))
-     SEP  (data_at sh node_type (vgamma2cdata (vgamma g1 l)) (pointer_val_val l))).
-  remember (vgamma g1 l) as dlr in |-*.
-  destruct dlr as [[dd ll] rr].
-  eapply semax_ram_seq;
-    [ subst RamFrame RamFrame0; unfold abbreviate;
-      repeat apply eexists_add_stats_cons; constructor
-    | load_tac 
-    | abbreviate_semax_ram].
-  replace (if dd then 1 else 0) with (if node_pred_dec (marked g1) l then 1 else 0).
-  Focus 2. {
-    destruct (node_pred_dec (marked g1)); destruct dd; auto; symmetry in Heqdlr.
-    apply vgamma_is_false in Heqdlr. simpl in a. unfold unmarked in Heqdlr. hnf in Heqdlr.
-    unfold Ensembles.In in Heqdlr. simpl in Heqdlr. apply Heqdlr in a. exfalso; auto.
-    apply vgamma_is_true in Heqdlr. exfalso; auto.
-  } Unfocus.
-  rewrite Heqdlr. simpl vgamma2cdata at 1.
-  assert ((Vint (Int.repr (if (@vlabel pointer_val (prod pointer_val LR) PointerVal_EqDec
-           PointerValLR_EqDec bool unit unit (@Graph_LGraph pSGG_VST bool unit unit g1)
-           l) then 1 else 0))) =
-          (Vint (Int.repr (if node_pred_dec (marked g1) l then 1 else 0)))). {
-    simpl. f_equal. f_equal.
-    change (vlabel (lg_gg g1) l) with (vlabel g1 l).
-    simpl.
-    destruct (@vlabel pointer_val (prod pointer_val LR) PointerVal_EqDec
-           PointerValLR_EqDec bool unit unit (@Graph_LGraph pSGG_VST bool unit unit g1)
-           l); auto.
-  }
-  rewrite H5. clear H5.
-  unlocalize
-    (PROP  ()
-     LOCAL (temp _root_mark (Vint (Int.repr (if node_pred_dec (marked g1) l then 1 else 0)));
-            temp _r (pointer_val_val r);
-            temp _l (pointer_val_val l);
-            temp _x (pointer_val_val x))
-     SEP  (graph sh x g1)).
-  Grab Existential Variables.
-  Focus 2. {
-    simplify_ramif.
-    destruct (vgamma g1 l) as [[dd ll] rr] eqn:? .
-    entailer!.
-    assert (vvalid g1 l). {
-      assert (weak_valid g1 l) by (eapply gamma_left_weak_valid; eauto).
-      destruct H5; auto. hnf in H5. subst. exfalso; intuition.
-    }
-    unfold vgamma2cdata.
-    apply (@va_reachable_internal_stable_ramify pSGG_VST _ _ _ (sSGG_VST sh) g1 x l (dd, ll, rr)); auto.
-    apply (gamma_left_reachable_included g1 _ _ _ _ H3 H_GAMMA_g1 l).
-    apply reachable_by_refl; auto.
-  } Unfocus.
-
-  (* if (root_mark == 0) { *)
-
-  unfold semax_ram.
-  apply semax_seq_skip.
-  Opaque node_pred_dec.
-  Opaque pSGG_VST.
-  (* remember (if node_pred_dec (marked g1) l then 1 else 0). *)
-  forward_if_tac
+  forward_if
     (EX g2: Graph,
      PROP  (edge_spanning_tree g1 (x, L) g2)
      LOCAL (temp _r (pointer_val_val r);
             temp _l (pointer_val_val l);
             temp _x (pointer_val_val x))
      SEP (vertices_at sh (reachable g1 x) g2)).
-
-  (* spanning(l); *)
-
-  Transparent node_pred_dec.
-  Transparent pSGG_VST.
-  destruct (node_pred_dec (marked g1) l). inversion H5.
-  localize
-    (PROP ()
-     LOCAL (temp _l (pointer_val_val l))
-     SEP (graph sh l g1)).
-  assert (vvalid g1 l). {
-    apply gamma_left_weak_valid in H1. 2: auto.
-    destruct H2.
-    rewrite (weak_valid_si _ _ _ s) in H1.
-    destruct H1. 2: auto.
-    hnf in H1. subst l.
-    simpl in H3. exfalso; auto.
-  }
-  assert (fst (fst (vgamma g1 l)) = false). {
-    simpl in n.
-    simpl. destruct (vlabel g1 l) eqn:? .
-    + symmetry in Heqb. apply n in Heqb. inversion Heqb.
-    + auto.
-  }
-  eapply semax_ram_seq';
-  [ subst RamFrame RamFrame0; unfold abbreviate;
-    repeat apply eexists_add_stats_cons; constructor
-  | semax_ram_call_body (sh, g1, l)
-  | semax_ram_after_call; intros g';
-    repeat (apply ram_extract_PROP; intro) ].
-  Focus 2. { gather_current_goal_with_evar. } Unfocus.
-  Focus 2. { gather_current_goal_with_evar. } Unfocus.
-  Focus 2. { gather_current_goal_with_evar. } Unfocus.
-  Focus 2. { gather_current_goal_with_evar. } Unfocus.
-  unlocalize
-    (PROP (edge_spanning_tree g1 (x, L) g')
-     LOCAL (temp _r (pointer_val_val r);
-            temp _l (pointer_val_val l);
-            temp _x (pointer_val_val x))
-     SEP (vertices_at sh (reachable g1 x) g'))
-    using [H8]%RamAssu
-    binding [g']%RamBind.
-  Grab Existential Variables.
-  Focus 2. {
-    assert (l = dst g1 (x, L)) by (simpl in H_GAMMA_g1; inversion H_GAMMA_g1; auto).
-    unfold edge_spanning_tree.
-    if_tac; subst l; [exfalso |]; auto.
-  } Unfocus.
-  Focus 1. {
-    unfold semax_ram. forward. entailer.
-    apply (exp_right g').
-    entailer.
-  } Unfocus.
-  Focus 1. {
-    simplify_ramif.
-    apply (@graph_ramify_aux1_left _ (sSGG_VST sh) _ g1 x true l r); auto.
-  } Unfocus.
-  gather_current_goal_with_evar.
-  gather_current_goal_with_evar.
-  gather_current_goal_with_evar.
-  destruct (node_pred_dec (marked g1) l). 2: exfalso; auto.
-
-  (* x -> l = 0; *)
-
-  localize
-   (PROP  ()
-    LOCAL (temp _x (pointer_val_val x))
-    SEP   (data_at sh node_type (Vint (Int.repr 1), (pointer_val_val l, pointer_val_val r))
-                   (pointer_val_val x))).
-  eapply semax_ram_seq';
-    [ subst RamFrame RamFrame0; unfold abbreviate;
-      repeat apply eexists_add_stats_cons; constructor
-    | store_tac 
-    | abbreviate_semax_ram].
-  cbv beta zeta iota delta [replace_nth].
-  change (@field_at CompSpecs sh node_type []
-           (Vint (Int.repr 1), (Vint (Int.repr 0), pointer_val_val r))) with
-         (@data_at CompSpecs sh node_type
-                   (Vint (Int.repr 1), (Vint (Int.repr 0), pointer_val_val r))).
-  unlocalize
-    (PROP ()
-     LOCAL (temp _r (pointer_val_val r);
-            temp _l (pointer_val_val l);
-            temp _x (pointer_val_val x))
-     SEP (vertices_at sh (reachable g1 x) (Graph_gen_left_null g1 x))).
-  Grab Existential Variables.
-  Focus 2. {
-    simplify_ramif.
-    apply (@graph_gen_left_null_ramify _ (sSGG_VST sh) g1 x true l r); auto.
-  } Unfocus.
-  Focus 1. {
-    unfold semax_ram. forward.
-    entailer.
-    apply (exp_right (Graph_gen_left_null g1 x)).
-    entailer!.
-    apply (edge_spanning_tree_left_null g1 x true l r); auto.
-    apply derives_refl.
-  } Unfocus.
-  Focus 1. {
-    forward.
-    Intro x0.
-    apply (exp_right x0).
-    entailer!.
-  } Unfocus.
-  Focus 2. {
-    forward.
-    entailer.
-    apply (exp_right g1).
-    entailer!; auto.
-    apply edge_spanning_tree_invalid.
+  - apply denote_tc_test_eq_split. 2: entailer!. apply (graph_left_local_facts _ _ _ true l r); auto.
+  - (* root_mark = l -> m; *)
+    localize [data_at sh node_type (vgamma2cdata (vgamma g1 l)) (pointer_val_val l)].
+    remember (vgamma g1 l) as dlr in |-*.
+    destruct dlr as [[dd ll] rr]. 
+    forward. simpl vgamma2cdata at 1.
+    replace (if dd then 1 else 0) with (if node_pred_dec (marked g1) l then 1 else 0).
+    Focus 2. {
+      destruct (node_pred_dec (marked g1)); destruct dd; auto; symmetry in Heqdlr.
+      apply vgamma_is_false in Heqdlr. simpl in a. unfold unmarked in Heqdlr. hnf in Heqdlr.
+      unfold Ensembles.In in Heqdlr. simpl in Heqdlr. apply Heqdlr in a. exfalso; auto.
+      apply vgamma_is_true in Heqdlr. exfalso; auto.
+    } Unfocus.
+    rewrite Heqdlr. clear dd ll rr Heqdlr.
+    unlocalize [graph sh x g1].
+    + destruct (vgamma g1 l) as [[dd ll] rr] eqn:? .
+      assert (vvalid g1 l). {
+        assert (weak_valid g1 l) by (eapply gamma_left_weak_valid; eauto).
+        destruct H5; auto. hnf in H5. subst. exfalso; intuition.
+      } unfold vgamma2cdata.
+      apply (@va_reachable_internal_stable_ramify pSGG_VST _ _ _ (sSGG_VST sh) g1 x l (dd, ll, rr)); auto.
+      apply (gamma_left_reachable_included g1 _ _ _ _ H3 H_GAMMA_g1 l).
+      apply reachable_by_refl; auto.
+    + (* if (root_mark == 0) { *)
+      Opaque node_pred_dec.
+      Opaque pSGG_VST.
+      (* remember (if node_pred_dec (marked g1) l then 1 else 0). *)
+      forward_if
+        (EX g2: Graph,
+         PROP  (edge_spanning_tree g1 (x, L) g2)
+         LOCAL (temp _r (pointer_val_val r);
+                temp _l (pointer_val_val l);
+                temp _x (pointer_val_val x))
+         SEP (vertices_at sh (reachable g1 x) g2)).
+      * (* spanning(l); *)
+        Transparent node_pred_dec.
+        Transparent pSGG_VST.
+        destruct (node_pred_dec (marked g1) l). 1: inversion H5.
+        localize [graph sh l g1].
+        assert (vvalid g1 l). {
+          apply gamma_left_weak_valid in H1. 2: auto.
+          destruct H2.
+          rewrite (weak_valid_si _ _ _ H2) in H1.
+          destruct H1. 2: auto.
+          hnf in H1. subst l.
+          simpl in H4. exfalso; auto.
+        } assert (fst (fst (vgamma g1 l)) = false). {
+          simpl in n.
+          simpl. destruct (vlabel g1 l) eqn:? ; auto.
+          symmetry in Heqb. apply n in Heqb. inversion Heqb.
+        } forward_call (sh, g1, l).
+        Intros g'.
+        unlocalize [vertices_at sh (reachable g1 x) g'] using g' assuming H8.
+        1: apply (@graph_ramify_aux1_left _ (sSGG_VST sh) g1 x true l r); auto.
+        Exists g'. entailer!.
+        assert (l = dst g1 (x, L)) by (simpl in H_GAMMA_g1; inversion H_GAMMA_g1; auto).
+        unfold edge_spanning_tree. if_tac; subst l; [exfalso |]; auto.
+      * (* x -> l = 0; *)
+        destruct (node_pred_dec (marked g1) l). 2: exfalso; auto.
+        localize [data_at sh node_type (Vint (Int.repr 1), (pointer_val_val l, pointer_val_val r)) (pointer_val_val x)].
+        forward.
+        unlocalize [vertices_at sh (reachable g1 x) (Graph_gen_left_null g1 x)].
+        1: apply (@graph_gen_left_null_ramify _ (sSGG_VST sh) g1 x true l r); auto.
+        Exists (Graph_gen_left_null g1 x).
+        entailer!.
+        apply (edge_spanning_tree_left_null g1 x true l r); auto.
+  - forward. Exists g1. entailer!. 2: apply derives_refl. apply edge_spanning_tree_invalid.
     + apply (@left_valid _ _ _ _ _ _ g1 _ _) in H3; auto.
     + intro. apply (valid_not_null g1 l).
-      - assert (l = dst g1 (x, L)) by (simpl in H_GAMMA_g1; inversion H_GAMMA_g1; auto).
-        rewrite H9. apply H8.
-      - hnf. apply (destruct_pointer_val_NP). left; auto.
-  } Unfocus.
-
-  (* if (r) { *)
-
-  Intro g2.
-  normalize.
-  assert (vvalid g2 x) by (rewrite <- (edge_spanning_tree_left_vvalid g1 g2 x); auto).
-  destruct (edge_spanning_tree_left_vgamma g1 g2 x l r H3 H_GAMMA_g1 H4) as [l' H_GAMMA_g2].
-
-  forward_if_tac
-    (EX g3: Graph,
-     PROP  (edge_spanning_tree g2 (x, R) g3)
-     LOCAL (temp _r (pointer_val_val r);
-            temp _l (pointer_val_val l);
-            temp _x (pointer_val_val x))
-     SEP (vertices_at sh (reachable g1 x) g3)); [  apply ADMIT (* type checking for pointer comparable. VST will fix it. *)
- | | gather_current_goal_with_evar ..].
-
-  (* root_mark = r -> m; *)
-
-  localize
-    (PROP  ()
-     LOCAL  (temp _r (pointer_val_val r))
-     SEP  (data_at sh node_type (vgamma2cdata (vgamma g2 r)) (pointer_val_val r))).
-  remember (vgamma g2 r) as dlr in |-*.
-  destruct dlr as [[dd ll] rr].
-  eapply semax_ram_seq;
-    [ subst RamFrame RamFrame0; unfold abbreviate;
-      repeat apply eexists_add_stats_cons; constructor
-    | load_tac 
-    | abbreviate_semax_ram].
-  replace (if dd then 1 else 0) with (if node_pred_dec (marked g2) r then 1 else 0).
-  Focus 2. {
-    destruct (node_pred_dec (marked g2)); destruct dd; auto; symmetry in Heqdlr.
-    apply vgamma_is_false in Heqdlr. simpl in a. unfold unmarked in Heqdlr. hnf in Heqdlr.
-    unfold Ensembles.In in Heqdlr. simpl in Heqdlr. apply Heqdlr in a. exfalso; auto.
-    apply vgamma_is_true in Heqdlr. exfalso; auto.
-  } Unfocus.
-  rewrite Heqdlr. simpl vgamma2cdata at 1.
-  assert ((Vint (Int.repr (if (@vlabel pointer_val (prod pointer_val LR) PointerVal_EqDec
-           PointerValLR_EqDec bool unit unit (@Graph_LGraph pSGG_VST bool unit unit g2)
-           r) then 1 else 0)))
-          = (Vint (Int.repr (if node_pred_dec (marked g2) r then 1 else 0)))). {
-    simpl. do 2 f_equal.
-    destruct (@vlabel pointer_val (prod pointer_val LR) PointerVal_EqDec
-           PointerValLR_EqDec bool unit unit (@Graph_LGraph pSGG_VST bool unit unit g2)
-           r); auto.
-  } rewrite H7. clear H7.
-  unlocalize
-    (PROP  ()
-     LOCAL (temp _root_mark (Vint (Int.repr (if node_pred_dec (marked g2) r then 1 else 0)));
-            temp _r (pointer_val_val r);
-            temp _l (pointer_val_val l);
-            temp _x (pointer_val_val x))
-     SEP  (vertices_at sh (reachable g1 x) g2)).
-  Grab Existential Variables.
-  Focus 2. {
-    simplify_ramif.
-    destruct (vgamma g2 r) as [[dd ll] rr] eqn:? .
-    assert (vvalid g1 r). {
-      assert (weak_valid g1 r) by (eapply gamma_right_weak_valid; eauto).
-      destruct H7; auto. hnf in H7; subst. exfalso; intuition.
-    }
-    unfold vgamma2cdata;
-    apply (@vertices_at_ramif_1_stable _ _ _ _ _ _ _ (SGA_VST sh) _ _ r (dd, ll, rr)); auto.
-    apply (gamma_right_reachable_included g1 _ _ _ _ H3 H_GAMMA_g1 r).
-    apply reachable_by_refl; auto.
-  } Unfocus.
-
-  (* if (root_mark == 0) { *)
-
-  unfold semax_ram.
-  apply semax_seq_skip.
-  Opaque node_pred_dec.
-  Opaque pSGG_VST.
-
-  forward_if_tac
-    (EX g3: Graph,
-     PROP  (edge_spanning_tree g2 (x, R) g3)
-     LOCAL (temp _r (pointer_val_val r);
-            temp _l (pointer_val_val l);
-            temp _x (pointer_val_val x))
-     SEP (vertices_at sh (reachable g1 x) g3)).
-
-  (* spanning(r); *)
-
-  Transparent node_pred_dec.
-  Transparent pSGG_VST.
-  destruct (node_pred_dec (marked g2) r). inversion H7.
-  localize
-    (PROP ()
-     LOCAL (temp _r (pointer_val_val r))
-     SEP (graph sh r g2)).
-  assert (vvalid g1 r). {
-      assert (weak_valid g1 r) by (eapply gamma_right_weak_valid; eauto).
-      destruct H8; auto. hnf in H8; subst. exfalso; intuition.
-  }
-  assert (vvalid g2 r) by (rewrite <- (edge_spanning_tree_left_vvalid g1 g2 x); auto).
-  assert (fst (fst (vgamma g2 r)) = false). {
-    simpl in n |-* . destruct (vlabel g2 r) eqn:? .
-    + symmetry in Heqb. apply n in Heqb. exfalso; auto.
-    + auto.
-  }
-  eapply semax_ram_seq';
-  [ subst RamFrame RamFrame0; unfold abbreviate;
-    repeat apply eexists_add_stats_cons; constructor
-  | semax_ram_call_body (sh, g2, r)
-  | semax_ram_after_call; intros g3;
-    repeat (apply ram_extract_PROP; intro) ].
-  
-  Focus 2. { gather_current_goal_with_evar. } Unfocus.
-  Focus 2. { gather_current_goal_with_evar. } Unfocus.
-  Focus 2. { gather_current_goal_with_evar. } Unfocus.
-  Focus 2. { gather_current_goal_with_evar. } Unfocus.
-  unlocalize
-    (PROP (edge_spanning_tree g2 (x, R) g3)
-     LOCAL (temp _r (pointer_val_val r);
-            temp _l (pointer_val_val l);
-            temp _x (pointer_val_val x))
-     SEP (vertices_at sh (reachable g1 x) g3))
-    using [H11]%RamAssu
-    binding [g3]%RamBind.
-  Grab Existential Variables.
-  Focus 2. {
-    assert (r = dst g2 (x, R)) by (simpl in H_GAMMA_g2; inversion H_GAMMA_g2; auto).
-    unfold edge_spanning_tree.
-    if_tac; subst r; [exfalso |]; auto.
-  } Unfocus.
-  Focus 1. {
-    unfold semax_ram.
-    forward.
-    entailer.
-    apply (exp_right g3).
-    entailer.
-  } Unfocus.
-  Focus 1. {
-    simplify_ramif.
-    apply (@graph_ramify_aux1_right _ (sSGG_VST sh) _ g1 g2 x l r); auto.
-  } Unfocus.
-  gather_current_goal_with_evar.
-  gather_current_goal_with_evar.
-  gather_current_goal_with_evar.
-  destruct (node_pred_dec (marked g2) r). 2: exfalso; auto.
-
-  (* x -> r = 0; *)
-  
-  localize
-   (PROP  ()
-    LOCAL (temp _x (pointer_val_val x))
-    SEP   (data_at sh node_type (Vint (Int.repr 1), (pointer_val_val l', pointer_val_val r))
-                     (pointer_val_val x))).
-  eapply semax_ram_seq';
-    [ subst RamFrame RamFrame0; unfold abbreviate;
-      repeat apply eexists_add_stats_cons; constructor
-    | store_tac 
-    | abbreviate_semax_ram].
-  cbv beta zeta iota delta [replace_nth].
-  change (@field_at CompSpecs sh node_type []
-           (Vint (Int.repr 1), (pointer_val_val l', Vint (Int.repr 0)))) with
-         (@data_at CompSpecs sh node_type
-                   (Vint (Int.repr 1), (pointer_val_val l', Vint (Int.repr 0)))).
-  unlocalize
-    (PROP ()
-     LOCAL (temp _r (pointer_val_val r);
-            temp _l (pointer_val_val l);
-            temp _x (pointer_val_val x))
-     SEP (vertices_at sh (reachable g1 x) (Graph_gen_right_null g2 x))).
-  Grab Existential Variables.
-  Focus 2. {
-    simplify_ramif.
-    apply (@graph_gen_right_null_ramify _ (sSGG_VST sh) g1 g2 x true l' r); auto.
-  } Unfocus.
-  Focus 1. {
-    unfold semax_ram. forward.
-    entailer.
-    apply (exp_right (Graph_gen_right_null g2 x)).
-    entailer!.
-    apply (edge_spanning_tree_right_null g2 x true l' r); auto.
-    apply derives_refl.
-  } Unfocus.
-  Focus 1. {
-    forward.
-    Intro x0.
-    apply (exp_right x0).
-    entailer!.
-  } Unfocus.
-  Focus 2. {
-    forward.
-    entailer.
-    apply (exp_right g2).
-    entailer!.
-    apply edge_spanning_tree_invalid.
-    + apply (@right_valid _ _ _ _ _ _ g2 _ _) in H5; auto.
-    + intro. apply (valid_not_null g2 r).
-      - assert (r = dst g2 (x, R)) by (simpl in H_GAMMA_g2; inversion H_GAMMA_g2; auto).
-        rewrite H11. apply H10.
-      - hnf; apply (destruct_pointer_val_NP). left; auto.
-  } Unfocus.
-
-  (* return *)
-  Intro g3.
-  normalize.
-  forward.
-  apply (exp_right g3).
-  entailer!.
-  Focus 2. {
-    destruct H2.
-    apply derives_refl'.
-    apply vertices_at_Same_set.
-    rewrite H2; reflexivity.
-  } Unfocus.
-  apply (edge_spanning_tree_spanning_tree g g1 g2 g3 x l r); auto. (* 1 min   27 sec *)
-Time Qed. (* 5500 sec *)
+      * assert (l = dst g1 (x, L)) by (simpl in H_GAMMA_g1; inversion H_GAMMA_g1; auto). rewrite H9. apply H8.
+      * hnf. destruct l. 1: inversion H4. auto.
+  - (* if (r) { *)
+    Intros g2.
+    assert (vvalid g2 x) by (rewrite <- (edge_spanning_tree_left_vvalid g1 g2 x); auto).
+    destruct (edge_spanning_tree_left_vgamma g1 g2 x l r H3 H_GAMMA_g1 H4) as [l' H_GAMMA_g2].
+    forward_if
+      (EX g3: Graph,
+       PROP  (edge_spanning_tree g2 (x, R) g3)
+       LOCAL (temp _r (pointer_val_val r);
+              temp _l (pointer_val_val l);
+              temp _x (pointer_val_val x))
+       SEP (vertices_at sh (reachable g1 x) g3)).
+    + apply denote_tc_test_eq_split. 2: entailer!. apply (graph_right_local_facts _ _ _ _ l l' r); auto.
+    + (* root_mark = r -> m; *)
+      localize [data_at sh node_type (vgamma2cdata (vgamma g2 r)) (pointer_val_val r)].
+      remember (vgamma g2 r) as dlr in |-*. destruct dlr as [[dd ll] rr].
+      forward. simpl vgamma2cdata at 1.
+      replace (if dd then 1 else 0) with (if node_pred_dec (marked g2) r then 1 else 0).
+      Focus 2. {
+        destruct (node_pred_dec (marked g2)); destruct dd; auto; symmetry in Heqdlr.
+        apply vgamma_is_false in Heqdlr. simpl in a. unfold unmarked in Heqdlr. hnf in Heqdlr.
+        unfold Ensembles.In in Heqdlr. simpl in Heqdlr. apply Heqdlr in a. exfalso; auto.
+        apply vgamma_is_true in Heqdlr. exfalso; auto.
+      } Unfocus. rewrite Heqdlr. clear dd ll rr Heqdlr.
+      unlocalize [vertices_at sh (reachable g1 x) g2].
+      * destruct (vgamma g2 r) as [[dd ll] rr] eqn:? .
+        assert (vvalid g1 r). {
+          assert (weak_valid g1 r) by (eapply gamma_right_weak_valid; eauto).
+          destruct H7; auto. hnf in H7; subst. exfalso; intuition.
+        } unfold vgamma2cdata; apply (@vertices_at_ramif_1_stable _ _ _ _ _ _ _ (SGA_VST sh) _ _ r (dd, ll, rr)); auto.
+        apply (gamma_right_reachable_included g1 _ _ _ _ H3 H_GAMMA_g1 r).
+        apply reachable_by_refl; auto.
+      * (* if (root_mark == 0) { *)
+        Opaque node_pred_dec.
+        Opaque pSGG_VST.
+        forward_if_tac
+          (EX g3: Graph,
+           PROP  (edge_spanning_tree g2 (x, R) g3)
+           LOCAL (temp _r (pointer_val_val r);
+                  temp _l (pointer_val_val l);
+                  temp _x (pointer_val_val x))
+           SEP (vertices_at sh (reachable g1 x) g3)).
+        -- (* spanning(r); *)
+          Transparent node_pred_dec.
+          Transparent pSGG_VST.
+          destruct (node_pred_dec (marked g2) r). 1: inversion H7.
+          localize [graph sh r g2].
+          assert (vvalid g1 r). {
+            assert (weak_valid g1 r) by (eapply gamma_right_weak_valid; eauto).
+            destruct H8; auto. hnf in H8; subst. exfalso; intuition.
+          }
+          assert (vvalid g2 r) by (rewrite <- (edge_spanning_tree_left_vvalid g1 g2 x); auto).
+          assert (fst (fst (vgamma g2 r)) = false). {
+            simpl in n |-* . destruct (vlabel g2 r) eqn:? ; auto.
+            symmetry in Heqb. apply n in Heqb. exfalso; auto.
+          }
+          forward_call (sh, g2, r).
+          Intros g3.
+          unlocalize [vertices_at sh (reachable g1 x) g3] using g3 assuming H11.
+          1: apply (@graph_ramify_aux1_right _ (sSGG_VST sh) g1 g2 x l r); auto.
+          Exists g3. entailer!.
+          assert (r = dst g2 (x, R)) by (simpl in H_GAMMA_g2; inversion H_GAMMA_g2; auto).
+          unfold edge_spanning_tree. if_tac; subst r; [exfalso |]; auto.
+        -- (* x -> r = 0; *)
+          destruct (node_pred_dec (marked g2) r). 2: exfalso; auto.
+          localize [data_at sh node_type (Vint (Int.repr 1), (pointer_val_val l', pointer_val_val r)) (pointer_val_val x)].
+          forward.
+          unlocalize [vertices_at sh (reachable g1 x) (Graph_gen_right_null g2 x)].
+          1: apply (@graph_gen_right_null_ramify _ (sSGG_VST sh) g1 g2 x true l' r); auto.
+          Exists (Graph_gen_right_null g2 x).
+          entailer!. apply (edge_spanning_tree_right_null g2 x true l' r); auto.
+    + forward. Exists g2. entailer!. apply edge_spanning_tree_invalid.
+      * apply (@right_valid _ _ _ _ _ _ g2 _ _) in H5; auto.
+      * intro. apply (valid_not_null g2 r).
+        -- assert (r = dst g2 (x, R)) by (simpl in H_GAMMA_g2; inversion H_GAMMA_g2; auto). rewrite H11. apply H10.
+        -- hnf. destruct r. 1: inversion H6. auto.
+    + (* return *)
+      Intros g3. forward. Exists g3. entailer!.
+      * apply (edge_spanning_tree_spanning_tree g g1 g2 g3 x l r); auto.
+      * destruct H2. apply derives_refl'. apply vertices_at_Same_set. rewrite H2; reflexivity.
+Qed. (* original: 5500 sec, VST 2.*: 8.91 secs *)
