data_structure/spatial_graph_unaligned_bi_VST.v
@@ -1,13 +1,7 @@
-Require Import RamifyCoq.msl_ext.abs_addr.
-Require Import RamifyCoq.msl_ext.seplog.
 Require Import RamifyCoq.msl_application.Graph.
 Require Import RamifyCoq.msl_application.GraphBi.
 Require Import VST.veric.SeparationLogic.
-Require Import RamifyCoq.veric_ext.SeparationLogic.
-Require Import RamifyCoq.msl_ext.alg_seplog.
 Require Import RamifyCoq.sample_mark.env_dispose_bi.
-Require Import RamifyCoq.veric_ext.SeparationLogic.
-Require Import RamifyCoq.floyd_ext.DataatSL.
 Require Import RamifyCoq.floyd_ext.share.
 
 Local Open Scope logic.
@@ -30,7 +24,8 @@ Instance SGBA_VST: PointwiseGraphBasicAssum pointer_val (pointer_val * LR).
 Defined.
 
 Instance pSGG_VST: pPointwiseGraph_Graph_Bi.
-  refine (Build_pPointwiseGraph_Graph_Bi pointer_val NullPointer mpred _).
+refine (Build_pPointwiseGraph_Graph_Bi pointer_val NullPointer
+                                       _).
 Defined.
 
 Definition vgamma2cdata (dlr : bool * addr * addr) : reptype node_type :=
@@ -41,10 +36,11 @@ Definition vgamma2cdata (dlr : bool * addr * addr) : reptype node_type :=
 Definition trinode (sh: share) (p: addr) (dlr: bool * addr * addr): mpred :=
   data_at sh node_type (vgamma2cdata dlr) (pointer_val_val p).
 
-Instance SGP_VST (sh: share) : PointwiseGraphPred addr (addr * LR) (bool * addr * addr) unit pred.
+Instance SGP_VST (sh: share) : PointwiseGraphPred addr (addr * LR) (bool * addr * addr) unit mpred.
   refine (Build_PointwiseGraphPred _ _ _ _ _ (trinode sh) (fun _ _ => emp)).
 Defined.
 
+(*
 Instance MSLstandard sh : MapstoSepLog (AAV (SGP_VST sh)) (trinode sh).
 Proof.
   intros.
@@ -56,8 +52,8 @@ Proof.
   unfold trinode.
   apply data_at_memory_block.
 Defined.
-
-Lemma sepcon_unique_vertex_at sh: writable_share sh -> sepcon_unique2 (@vertex_at _ _ _ _ _ (SGP_VST sh)).
+*)
+Lemma sepcon_unique_vertex_at sh: writable_share sh -> iter_sepcon.sepcon_unique2 (@vertex_at _ _ _ _ _ (SGP_VST sh)).
 Proof.
   intros.
   hnf; intros.
@@ -67,11 +63,8 @@ Proof.
   rewrite data_at_isptr.
   normalize.
   apply data_at_conflict.
-  + apply sepalg.nonidentity_nonunit.
-    apply readable_nonidentity, writable_readable.
-    auto.
-  + change (sizeof node_type) with 12.
-    apply pointer_range_overlap_refl; auto; omega.
+  + apply readable_nonidentity, writable_readable. auto.
+  + change (sizeof node_type) with 12. omega.
 Qed.
 
 (*
@@ -145,6 +138,5 @@ Instance SGAvn_VST (sh: wshare): PointwiseGraphAssum_vn (SGP_VST sh) NullPointer
 Defined.
 
 Instance sSGG_VST (sh: wshare): @sPointwiseGraph_Graph_Bi pSGG_VST bool unit.
-  refine (Build_sPointwiseGraph_Graph_Bi pSGG_VST _ _ (SGP_VST sh) (SGA_VST sh) (SGAvs_VST sh) (SGAvn_VST sh)).
+  refine (Build_sPointwiseGraph_Graph_Bi pSGG_VST _ _ _ (SGP_VST sh) (SGA_VST sh) (SGAvs_VST sh) (SGAvn_VST sh)).
 Defined.
-
