msl_application/ArrayGraph.v
@@ -10,8 +10,6 @@ Require Import RamifyCoq.lib.Ensembles_ext.
 Require Import RamifyCoq.lib.EquivDec_ext.
 Require Import RamifyCoq.lib.Relation_ext.
 Require Import RamifyCoq.lib.List_ext.
-Require Import RamifyCoq.msl_ext.abs_addr.
-Require Import RamifyCoq.msl_ext.seplog.
 Require Import RamifyCoq.graph.graph_model.
 Require Import RamifyCoq.graph.weak_mark_lemmas.
 Require Import RamifyCoq.graph.path_lemmas.
