msl_application/GList_UnionFind.v
@@ -7,7 +7,6 @@ Require Import RamifyCoq.lib.Coqlib.
 Require Import RamifyCoq.lib.Ensembles_ext.
 Require Import RamifyCoq.lib.EquivDec_ext.
 Require Import RamifyCoq.lib.Relation_ext.
-Require Import RamifyCoq.msl_ext.seplog.
 Require Import RamifyCoq.graph.graph_model.
 Require Import RamifyCoq.graph.path_lemmas.
 Require Import RamifyCoq.graph.graph_gen.
