msl_application/GraphBi_Copy.v
@@ -8,8 +8,6 @@ Require Import RamifyCoq.lib.Coqlib.
 Require Import RamifyCoq.lib.EquivDec_ext.
 Require Import RamifyCoq.lib.relation_list.
 Require Import RamifyCoq.lib.Morphisms_ext.
-Require Import RamifyCoq.msl_ext.abs_addr.
-Require Import RamifyCoq.msl_ext.seplog.
 Require Import RamifyCoq.msl_ext.log_normalize.
 Require Import RamifyCoq.msl_ext.iter_sepcon.
 Require Import RamifyCoq.graph.graph_model.
@@ -27,7 +25,6 @@ Require Import RamifyCoq.msl_application.Graph.
 Require Import RamifyCoq.msl_application.GraphBi.
 Require Import RamifyCoq.msl_application.Graph_Copy.
 Require Import Coq.Logic.Classical.
-Import RamifyCoq.msl_ext.seplog.OconNotation.
 
 Open Scope logic.
 
