msl_application/Graph_Copy.v
@@ -6,8 +6,6 @@ Require Import RamifyCoq.lib.EquivDec_ext.
 Require Import RamifyCoq.lib.List_ext.
 Require Import RamifyCoq.lib.relation_list.
 Require Import RamifyCoq.lib.Morphisms_ext.
-Require Import RamifyCoq.msl_ext.abs_addr.
-Require Import RamifyCoq.msl_ext.seplog.
 Require Import RamifyCoq.msl_ext.log_normalize.
 Require Import RamifyCoq.msl_ext.iter_sepcon.
 Require Import RamifyCoq.msl_ext.ramification_lemmas.
@@ -24,7 +22,6 @@ Require Import RamifyCoq.graph.graph_morphism.
 Require Import RamifyCoq.graph.local_graph_copy.
 Require Import RamifyCoq.msl_application.Graph.
 Require Import Coq.Logic.Classical.
-Import RamifyCoq.msl_ext.seplog.OconNotation.
 
 Local Open Scope logic.
 
@@ -797,5 +794,3 @@ Proof.
 Qed.
 
 End PointwiseGraph_Copy.
-
-
