msl_ext/log_normalize.v
@@ -1,5 +1,3 @@
-Require Import RamifyCoq.msl_ext.abs_addr.
-Require Import RamifyCoq.msl_ext.seplog.
 Require Import VST.msl.Extensionality.
 Require Import VST.msl.simple_CCC.
 Require Import VST.msl.seplog.
@@ -119,6 +117,7 @@ Proof.
   auto.
 Qed.
 
+(*
 Lemma ocon_sep_true: forall {A} `{OverlapSepLog A} (P Q: A), ocon P Q |-- P * TT.
 Proof.
   intros.
@@ -127,6 +126,7 @@ Proof.
   + rewrite ocon_TT.
     apply derives_refl.
 Qed.
+*)
 
 Lemma exp_allp: forall {A} `{NatDed A} (S T: Type) (P: S -> T -> A),
     exp (fun s => allp (P s)) |-- allp (fun t => exp (fun s => P s t)).
@@ -148,6 +148,7 @@ Proof.
   apply H.
 Qed.
 
+(*
 Lemma precise_andp_left: forall {A} `{PreciseSepLog A} P Q, precise P -> precise (P && Q).
 Proof.
   intros.
@@ -225,6 +226,7 @@ Proof.
       specialize (H0 (ex_intro _ x H3)); tauto.
     - apply FF_precise.
 Qed.
+ *)
 
 Lemma exp_sepcon: forall {A} `{SepLog A} {B} (P Q: B -> A), exp (P * Q) |-- exp P * exp Q.
 Proof.
@@ -243,6 +245,7 @@ Proof.
   apply modus_ponens_wand.
 Qed.
 
+(*
 Lemma precise_left_sepcon_andp_sepcon: forall {A} `{PreciseSepLog A} P Q R, precise P -> (P * Q) && (P * R) |-- P * (Q && R).
 Proof.
   intros.
@@ -438,6 +441,7 @@ Proof.
   eapply CCC_exp_prod2.
   apply ocon_owand_CCC.
 Qed.
+ *)
 
 (* Can be moved into VST/msl/log_normalize. *)
 Lemma CCC_expo_expo_comm': forall A prod expo {ND: NatDed A} {CCC: CCCviaNatDed A prod expo},
@@ -477,6 +481,7 @@ Proof.
   apply sepcon_derives; auto.
 Qed.
 
+(*
 Ltac normalize_overlap :=
   repeat
     match goal with
@@ -492,6 +497,7 @@ Ltac normalize_overlap :=
     end;
   repeat rewrite <- andp_assoc;
   try normalize.
+ *)
 
 Lemma exp_emp: forall {A B} `{ClassicalSep B} (P: A -> B), EX x:A, P x * emp = EX x: A, P x.
 Proof.
@@ -501,15 +507,3 @@ Proof.
   rewrite sepcon_emp.
   auto.
 Qed.
-
-Goal forall {A} `{CorableOverlapSepLog A} P (Q R: A), ocon (!! P && !! P  && Q) R = ocon (!! P && Q && !! P) (!! P && R && !! P).
-intros.
-(* normalize_overlap. *)
-Abort.
-
-Goal forall {A} `{CorableOverlapSepLog A} P R (Q: A), Q |-- ocon (ocon (EX x: nat, P x) Q) (EX x: nat, R x).
-intros.
-(* normalize_overlap. *)
-(* apply (exp_right 0). *)
-(* normalize_overlap. *)
-Abort.
