sample_mark/env_garbage_collector.v
@@ -2,7 +2,7 @@ Require Export VST.floyd.proofauto.
 Require Export RamifyCoq.floyd_ext.semax_ram_lemmas.
 Require Export RamifyCoq.floyd_ext.exists_trick.
 Require Export RamifyCoq.floyd_ext.closed_lemmas.
-Require Export RamifyCoq.floyd_ext.comparable.
+(* Require Export RamifyCoq.floyd_ext.comparable. *)
 Require Export RamifyCoq.sample_mark.garbage_collector.
 
 Local Open Scope logic.
