sample_mark/spatial_graph_bi_copy.v
@@ -1,16 +1,8 @@
-Require Import RamifyCoq.msl_ext.abs_addr.
-Require Import RamifyCoq.msl_ext.seplog.
+Require Import RamifyCoq.msl_ext.iter_sepcon.
 Require Import RamifyCoq.msl_application.Graph.
 Require Import RamifyCoq.msl_application.GraphBi.
 Require Import VST.veric.SeparationLogic.
-Require Import RamifyCoq.veric_ext.SeparationLogic.
-Require Import RamifyCoq.msl_ext.alg_seplog.
 Require Import RamifyCoq.sample_mark.env_copy_bi.
-Require Import RamifyCoq.veric_ext.SeparationLogic.
-Require Import RamifyCoq.floyd_ext.DataatSL.
-Require Import RamifyCoq.floyd_ext.share.
-
-Local Open Scope logic.
 
 Section pSGG_VST.
 
@@ -34,7 +26,7 @@ Defined.
 End pSGG_VST.
 
 Instance pSGG_VST: pPointwiseGraph_Graph_Bi.
-  refine (Build_pPointwiseGraph_Graph_Bi pointer_val NullPointer mpred SGBA_VST).
+  refine (Build_pPointwiseGraph_Graph_Bi pointer_val NullPointer SGBA_VST).
 Defined.
 
 Section sSGG_VST.
@@ -46,10 +38,11 @@ Definition trinode (sh: share) (p: addr) (dlr: addr * addr * addr): mpred :=
                     (pointer_val_val p)
   end.
 
-Instance SGP_VST (sh: share) : PointwiseGraphPred addr (addr * LR) (addr * addr * addr) unit pred.
+Instance SGP_VST (sh: share) : PointwiseGraphPred addr (addr * LR) (addr * addr * addr) unit mpred.
   refine (Build_PointwiseGraphPred _ _ _ _ _ (trinode sh) (fun _ _ => emp)).
 Defined.
 
+(*
 Instance MSLstandard sh : MapstoSepLog (AAV (SGP_VST sh)) (trinode sh).
 Proof.
   intros.
@@ -61,6 +54,7 @@ Proof.
   unfold trinode.
   apply data_at_memory_block.
 Defined.
+ *)
 
 Lemma sepcon_unique_vertex_at sh: writable_share sh -> sepcon_unique2 (@vertex_at _ _ _ _ _ (SGP_VST sh)).
 Proof.
@@ -72,11 +66,8 @@ Proof.
   rewrite data_at_isptr.
   normalize.
   apply data_at_conflict.
-  + apply sepalg.nonidentity_nonunit.
-    apply readable_nonidentity, writable_readable.
-    auto.
-  + change (sizeof node_type) with 16.
-    apply pointer_range_overlap_refl; auto; omega.
+  + apply readable_nonidentity, writable_readable. auto.
+  + change (sizeof node_type) with 16. omega.
 Qed.
 
 (*
@@ -155,7 +146,7 @@ End sSGG_VST.
 Hint Extern 10 (@sepcon_unique2 _ _ _ _ _ (@vertex_at _ _ _ _ _ _)) => apply sepcon_unique_vertex_at; auto.
 
 Instance sSGG_VST (sh: wshare): @sPointwiseGraph_Graph_Bi pSGG_VST addr (addr * LR).
-  refine (Build_sPointwiseGraph_Graph_Bi pSGG_VST _ _ (SGP_VST sh) (SGA_VST sh) (SGAvs_VST sh) (SGAvn_VST sh)).
+  refine (Build_sPointwiseGraph_Graph_Bi pSGG_VST _ _ _ (SGP_VST sh) (SGA_VST sh) (SGAvs_VST sh) (SGAvn_VST sh)).
 Defined.
 
 Global Opaque pSGG_VST sSGG_VST.
